State

DenotationalLean/ADeriv.lean
@@ -1,12 +1,12 @@
 
 import DenotationalLean.Imp
+import DenotationalLean.State
 
-abbrev State := Loc -> Nat
 abbrev Config := Aexp × State
 
 inductive a_deriv : Config -> Nat -> Prop
   | num {n σ} : a_deriv (Aexp.Nat n, σ) n
-  | loc {l σ} : a_deriv (Aexp.Loc l, σ) (σ l)
+  | loc {l σ} : a_deriv (Aexp.Loc l, σ) (State.lookup σ l)
   | add {a0 n0 a1 n1 σ} : a_deriv (a0,σ) n0 -> a_deriv (a1,σ) n1 -> a_deriv (Aexp.Add a0 a1,σ) (n0+n1)
   | sub {a0 n0 a1 n1 σ} : a_deriv (a0,σ) n0 -> a_deriv (a1,σ) n1 -> a_deriv (Aexp.Sub a0 a1,σ) (n0-n1)
   | mul {a0 n0 a1 n1 σ} : a_deriv (a0,σ) n0 -> a_deriv (a1,σ) n1 -> a_deriv (Aexp.Mul a0 a1,σ) (n0*n1)
@@ -15,10 +15,10 @@ example : a_deriv
     (Aexp.Add
       (Aexp.Add (Aexp.Loc "Init") (Aexp.Nat 5))
       (Aexp.Add (Aexp.Nat 7) (Aexp.Nat 9)),
-    fun x => match x with | "Init" => 0 | _ => /- anything -/ 0)
+    [("Init",0)])
     21 := by
-  let σ := fun x => match x with | "Init" => 0 | _ => 0
-  have h0 : σ "Init" = 0 := by rfl
+  let σ := [("Init",0)]
+  have h0 : State.lookup σ "Init" = 0 := by rfl
   have hi := @a_deriv.loc "Init" σ
   simp [h0] at hi
   have h5 := @a_deriv.num 5 σ
