DenotationalLean/State.lean
@@ -1,0 +1,12 @@
+
+import DenotationalLean.Imp
+
+abbrev State := List (Loc × Nat)
+
+namespace State
+
+def lookup(σ : State) : Loc -> Nat := fun l => match σ with
+  | [] => 0
+  | ((l',n)::xs) => if l == l' then n else lookup xs l
+
+end State
